Add theorems for `Append.lean` (#221)
This adds theorems for the single implementation of the
`std::append::Append` trait contained in that file, and also for the
implementation of `std::slice::Slice::append` that it depends on.

stdlib/lampe/Stdlib/Append.lean
@@ -1,6 +1,55 @@
 import «std-1.0.0-beta.12».Extracted
 import Lampe
 
+import Stdlib.Slice
+
 namespace Lampe.Stdlib.Append
 
 open «std-1.0.0-beta.12»
+open Lampe.Stdlib
+
+set_option Lampe.pp.Expr true
+set_option Lampe.pp.STHoare true
+
+/-- A shorthand for a call to the `std::append::Append::empty` method. -/
+@[reducible]
+def empty {p}
+    (generics : HList Kind.denote «std-1.0.0-beta.12::append::Append».«#genericKinds»)
+    (Self : Tp)
+    (associatedTypes : HList Kind.denote «std-1.0.0-beta.12::append::Append».«#associatedTypesKinds»)
+    (fnGenerics : HList Kind.denote «std-1.0.0-beta.12::append::Append».«#genericKinds»)
+  : HList (Tp.denote p)
+      («std-1.0.0-beta.12::append::Append».empty.«#inputs» generics Self associatedTypes fnGenerics)
+  → Expr (Tp.denote p)
+      («std-1.0.0-beta.12::append::Append».empty.«#output» generics Self associatedTypes fnGenerics) :=
+  «std-1.0.0-beta.12::append::Append».empty generics Self associatedTypes fnGenerics
+
+/-- A shorthand for a call to the `std::append::Append::append` method. -/
+@[reducible]
+def append {p}
+    (generics : HList Kind.denote «std-1.0.0-beta.12::append::Append».«#genericKinds»)
+    (Self : Tp)
+    (associatedTypes : HList Kind.denote «std-1.0.0-beta.12::append::Append».«#associatedTypesKinds»)
+    (fnGenerics : HList Kind.denote «std-1.0.0-beta.12::append::Append».«#genericKinds»)
+  : HList (Tp.denote p)
+      («std-1.0.0-beta.12::append::Append».append.«#inputs» generics Self associatedTypes fnGenerics)
+  → Expr (Tp.denote p)
+      («std-1.0.0-beta.12::append::Append».append.«#output» generics Self associatedTypes fnGenerics) :=
+  «std-1.0.0-beta.12::append::Append».append generics Self associatedTypes fnGenerics
+
+theorem slice_empty_spec {p T }
+  : STHoare p env ⟦⟧
+    (empty h![] (Tp.slice T) h![] h![] h![])
+    (fun r => r = []) := by
+  resolve_trait
+  steps
+  simp_all
+
+theorem slice_append_spec {p T self other}
+  : STHoare p env ⟦⟧
+    (append h![] (Tp.slice T) h![] h![] h![self, other])
+    (fun r => r = self ++ other) := by
+  resolve_trait
+  steps [Slice.append_spec]
+  simp_all
+
